$R_{\mu\nu} = R^{\lambda}_{\ \mu\lambda\nu}$

$G_{\mu\nu} = R_{\mu\nu} - \frac{1}{2} g_{\mu\nu} R$

$\nabla_\mu T^{\mu\nu} = 0$

$
C_{\alpha\beta\gamma\delta} =
R_{\alpha\beta\gamma\delta}
- \frac{2}{n-2} \left(
    g_{\alpha[\gamma} R_{\delta]\beta}
    - g_{\beta[\gamma} R_{\delta]\alpha}
  \right)
+ \frac{2}{(n-1)(n-2)} R g_{\alpha[\gamma} g_{\delta]\beta}
$

$
\Box \phi = g^{\mu\nu} \nabla_\mu \nabla_\nu \phi
$

$
\Gamma^\rho_{\mu\nu} = \frac{1}{2} g^{\rho\sigma}
\left(
  \partial_\mu g_{\sigma\nu} + \partial_\nu g_{\sigma\mu} - \partial_\sigma g_{\mu\nu}
\right)
$

$
ds^2 = -\left(1-\frac{2M}{r}\right) dt^2 + \frac{dr^2}{1-2M/r} + r^2 d\theta^2 + r^2 \sin^2\theta\, d\phi^2
$

$
\Delta f = \frac{1}{r^2} \partial_r \left( r^2 \partial_r f \right)
+ \frac{1}{r^2\sin\theta} \partial_\theta \left( \sin\theta \partial_\theta f \right)
+ \frac{1}{r^2 \sin^2\theta} \partial^2_\phi f
$

$
K_{ij} = -\frac{1}{2\alpha} \left( \partial_t \gamma_{ij} - D_i \beta_j - D_j \beta_i \right)
$

$
\mathcal{L}_\xi g_{\mu\nu} = \xi^\alpha \partial_\alpha g_{\mu\nu} + g_{\alpha\nu} \partial_\mu \xi^\alpha + g_{\mu\alpha} \partial_\nu \xi^\alpha
$

$
R_{\mu\nu\alpha\beta} = -R_{\nu\mu\alpha\beta} = -R_{\mu\nu\beta\alpha} = R_{\nu\mu\beta\alpha}
$

$
\nabla_\sigma R^{\alpha}_{\ \beta\mu\nu}
+ \nabla_\nu R^{\alpha}_{\ \beta\sigma\mu}
+ \nabla_\mu R^{\alpha}_{\ \beta\nu\sigma} = 0
$

$
T^{\mu\nu} = (\rho + p) u^\mu u^\nu + p g^{\mu\nu}
$

$
S = \int d^4x \, \sqrt{-g}\; \mathcal{L}
$

$
h_{\mu\nu} = g_{\mu\nu} - \eta_{\mu\nu}
$

$
\delta R_{\mu\nu} = \nabla_\alpha \delta \Gamma^\alpha_{\mu\nu} - \nabla_\nu \delta \Gamma^\alpha_{\mu\alpha}
$

$
R = g^{\mu\nu} R_{\mu\nu}
$

$
\frac{d^2x^\mu}{d\tau^2} + \Gamma^\mu_{\nu\rho} \frac{dx^\nu}{d\tau} \frac{dx^\rho}{d\tau} = 0
$
